---
mathjax: true
---

## Problem 1

If $s_1,s_2, s_3$ are the sums of $n, 2n, 3n$ terms respectively of an arithmetical progression, shew that $s_3 = 3 (s_2 â€” s_1)$

## Solution

Let the terms of the arithmetic progression be $a, a+d, a+2d, ..., a+(n-1)d, .... , a+(2n-1)d, ...a+(3n-1)d$

Sum of the first $k$ terms is

  $$\begin{aligned}\label{eq1} \sum & = a+(a+d)+(a+2d)+...+(a+(k-1)d) & = ka + d(1+2+3+4+5+...+(k-1)) & = ka+d\frac{(k-1)k}{2}\end{aligned}$$

So $$\begin{aligned} s_2-s_1 & = (2n)a+d\frac{(2n-1)2n}{2} - (na+d\frac{(n-1)n}{2}) & = (2na-na)+d\frac{((2n-1)2-(n-1)n)}{2} & = na+d\frac{(4n^2-2n-n^2+n)}{2} & = na+d\frac{(3n^2-n)}{2} & = na+d\frac{(3n-1)n}{2} \end{aligned}$$

&

$$3(s_2-s_1) = 3na + \frac{(3n-1)3n}{2} $$ 

which is the same as subsituiting $3n$ for $k$ in the formula above

[Next](2.html)
