---
layout: post
tags: equations
---

## Problem

Solve the equations:

$ ax^2+bxy+cy^2=bx^2+cxy+ay^2=d $ [MATH. TRIPOS.]

## Solution

Set $y=mx$ and subtituiting in the first two equations we get
$$ \begin{align} ax^2+bx(mx)+c(mx)^2 &= bx^2+cx(mx)+a(mx)^2 \\
                 x^2(a+bm+cm^2) &= x^2(b+cm+am^2) \\
				 a+bm+cm^2 &= b+cm+am^2 \\
				 (c-a)m^2 + (b-c)m + (a-b) &= 0 \end{align} $$

Let $m_1, m_2$ be the roots of the above equation. 

$$ \begin{align} ax^2+bx(mx)+c(mx)^2 &= d \\
                 x^2(a+bm+cm^2) &=d \\
				 x &= \pm{\frac{d}{a+bm+cm^2}} \end{align} $$
				 
Subsituting for $m_1, m_2$ in the above equation gives 4 different values for $x$. 