---
layout: post
categories: equations
tags: equations
---

## Problem

Solve the equations
  1. $(x+2)(x+3)(x-4)(x-5)=44$
  2. $x(y+z)+2=0, y(z-2x)+21=0, z(2x-y)=5$

## Solution

  1. $(x+2)(x+3)(x-4)(x-5)=44$
  2. $x(y+z)+2=0, y(z-2x)+21=0, z(2x-y)=5$

     Add the second and third equations
     $$\begin{align} y(z-2x)+21&=0 \\
                     z(2x-y)&=5 \end{align}$$
     $$\begin{align} -2xy + 21 + 2xz &= 5 \\
                     -2x(y-z) &= -16 \\
                     x(y-z) &= 8 \end{align}$$

     Divide the first equation by the preceding one
     $$\begin{align} \frac{x(y+z)}{x(y-z)}&=\frac{-2}{8} \\
                     \frac{y+z}{y-z}&=\frac{-1}{4} \\
                  4y+4z &= -(y-z) \\
                     5y &= -3z \end{align}$$
     i.e $y=-\frac{3}{5}z$

     Subsituiting this in the first equation we get
     $$\begin{align} x(y+z)+2&=0 \\
                     x(-\frac{3}{5}z+z)+2&=0 \\
                     x(\frac{2}{5}z)&=-2 \\
                     xz &= -5 \end{align} $$

     Subsituiting this in the second equation we get
     $$\begin{align} z(2x-y)&=5 \\
                    2xz-yz&=5\\
                   2(-5)-(-\frac{3}{5}z)z&=5 \\
                  \frac{3}{5}z^2 & = 15 \\
                  z^2 &= 25 \\
                  z = \pm{5} \end{align} $$

     So the solutions are

     $ x =\mp{1}, y=\mp{3}, z=\pm{5} $
