---
layout: post
tags: equations
---

## Problem

If the equation $\frac{a}{x+a}+\frac{b}{x+b}=\frac{c}{x+c}+\frac{d}{x+d}$ have a pair of equal roots, then either one of the quantities $a$ or $b$ is equal to one of the quantities $c$ or $d$, or else $\frac{1}{a}+\frac{1}{b}=\frac{1}{c}+\frac{1}{d}$. Prove also that the roots are then $-a, -a, 0; -b, -b, 0;$ or $0,0,-\frac{2ab}{a+b}$. [Math Tripos]

## Solution

The equation can be rewritten as


$$\begin{align} 1-\frac{x}{x+a}+1-\frac{x}{x+b} &= 1-\frac{x}{x+c}+1-\frac{x}{x+d} \\
                 \frac{x}{x+a}+\frac{x}{x+b} &=\frac{x}{x+c}+\frac{x}{x+d} \\
                 \frac{x}{x+a}-\frac{x}{x+c} &=\frac{x}{x+d}-\frac{x}{x+b} \\
                 x\frac{c-a}{(x+a)(x+c)} &= x\frac{b-d}{(x+d)(x+b)} \end{align}$$

So $x=0$ is always a root and the equation becomes

$$\begin{align} \frac{c-a}{(x+a)(x+c)} &= \frac{b-d}{(x+d)(x+b)} \\
              (x+a)(x+c) &= \frac{(c-a)}{b-d}(x+d)(x+b)\end{align}$$

if $c=a$ and $b \ne d$ the RHS vanishes and the equation becomes

$$ (x+a)(x+a) = 0 $$

and the roots are $-a, -a$

Similarly if $b=d$ and $c \ne a$ the roots of the resulting equation become $-b,-b$

if $c \ne a$ and $b \ne d$ the equation becomes

$$\begin{align} \frac{(x+a)(x+c)}{c-a}=\frac{(x+b)(x+d)}{b-d} \end{align} $$

expanding and rearranging we get

$$\begin{align} x^2(\frac{1}{c-a}-\frac{1}{b-d})+x(\frac{a+c}{c-a}-\frac{d+b}{b-d}) + \frac{ac}{c-a}-\frac{db}{b-d} = 0 \end{align} $$

$x=0$ is already a root, for it to be a double root the 3rd time of above equation should be zero

$$\begin{align} 
         \frac{ac}{c-a}-\frac{db}{b-d} = 0 \\
		 \frac{ac}{c-a} = \frac{db}{b-d} \\
		 \frac{c-a}{ac} = \frac{b-d}{db} \\
		 \frac{1}{a}-\frac{1}{c} = \frac{1}{d} - \frac{1}{b} \\
		 \frac{1}{a}+\frac{1}{b} = \frac{1}{c} + \frac{1}{d} \\
\end{align} $$

and the other root would be 

$$\begin{align}
    x &= -\frac{\frac{a+c}{c-a}-\frac{d+b}{b-d}}{\frac{1}{c-a}-\frac{1}{b-d}} \\
	  &= -\frac{(a+c)(b-d)-(d+b)(c-a)}{b-d-(c-a)} \\
	  &= -\frac{ab-ad+bc-cd-(cd-ad+bc-ab)}{a+b-(c+d)} \\
	  &= -\frac{2ab-2cd}{a+b-(c+d)} \\
\end{align}$$

From the above equation $\frac{1}{a}+\frac{1}{b} = \frac{1}{c} + \frac{1}{d}$ i.e $ c+d = cd\frac{a+b}{ab}$ . Substituiting this we get
$$\begin{align}
    x &= -\frac{2ab-2cd}{a+b-(c+d)} \\
	  &= -\frac{2ab-2cd}{a+b-cd\frac{a+b}{ab}} \\
	  &= -2\frac{ab-cd}{(a+b)(1-\frac{cd}{ab})} \\
	  &= -\frac{2ab}{a+b}
\end{align}$$
