---
layout: post
tags: equations
---

## Extract the square root of

(1) $(a^2+ab+bc+ca)(bc+ca+ab+b^2)(bc+ca+ab+c^2)$

(2) $ 1 - x + \sqrt{22x-15-8x^2} $

## Solution

(1) The equation can be arranged as 

$(a^2+ab+bc+ca)(bc+ca+ab+b^2)(bc+ca+ab+c^2)$
$(a(a+b)+c(b+a))(c(a+b)+b(a+b))(b(c+a)+c(a+c))$
$(a+c)(a+b)(c+b)(a+b)(b+c)(c+a)$
	
So the square root is $(a+c)(a+b)(c+b)$

(2) Let the square root be of the form $\sqrt{a+bx}+\sqrt{c+dx}$. Squaring this we get
$(a+c)+(b+d)x+2\sqrt{(a+bx)(c+dx)}$ i.e $(a+c)+(b+d)x+\sqrt{4ac+4(bc+ad)x+4bdx^2}$

Comparing coeffs with the original equation we get
$$\begin{align} a +c = 1 \\
   b+d  = -1 \\
   4ac = -15 i.e ac=-\frac{15}{4} \\
   4bd=-8 i.e bd = -2 \\
   4(bc+ad)=22\\
  \end{align} $$
  
Solving for $b,d$ we get $b=-2, d=1$. For $a,c$ the solutions are the roots of $t^2-t-\frac{15}{4} = 0$ i.e 
$t = \frac{1\pm{\sqrt{1+4\frac{15}{4}}}}{2} = \frac{1\pm{4}}{2} = \frac{5}{2}, -\frac{3}{2}$

Using $b=-2, d=1$ in $4(bc+ad)=22$ we get $4(-2c+a)=22$ i.e $2a-4c = 11$ this is satisfied by $a=\frac{5}{2}, c=-\frac{3}{2}$

So the square root is $\sqrt{\frac{5}{2}-2x}+\sqrt{-\frac{3}{2}+x}$
