---
layout: post
tags: equations
---

## Problem

Solve the equations

1) $(a+b)(ax+b)(a-bx) = (a^2x-b^2)(a+bx))$

2) $x^\frac{1}{3} + (2x-3)^\frac{1}{3} = ({12(x-1)})^\frac{1}{3}$ [India Civil Service]

## Solution

1)  $(a+b)(ax+b)(a-bx) = (a^2x-b^2)(a+bx))$.

  By inspection we see that putting x equals 1 satisfies the above equation which means that $x=1$ is a root. 
  Rearranging the equation we see
  $$\begin{align} (a+b)(ax+b)(a-bx) &= (a^2x-b^2)(a+bx)) \\
                  (a+b)(a^2x-abx^2+ab-b^2x) &= (a^3x+a^2bx^2-ab^2-b^3x) \\
				  x^2(a^2b+ab(a+b))+x(a^3-b^3-(a+b)(a^2-b^2)) -ab^2-ab(a+b) &= 0 \\
				 \end{align}$$
				 
  So the product of the roots is $\frac{-ab^2-ab(a+b)}{a^2b+ab(a+b)}$. Since one of the roots is 1 this is the other root
     $$\begin{align} x &= \frac{-ab^2-a^2b-ab^2}{a^2b+a^2b+ab^2} \\
	                   &= -\frac{2ab^2+a^2b}{2a^2b+ab^2} \\
					   &= -\frac{2b+a}{2a+b} \\
	  \end{align} $$

2) $ x^\frac{1}{3} + (2x-3)^\frac{1}{3} = (12(x-1))^\frac{1}{3} $. By inspection putting x equals to 1 satisfies the above equation which means that it is a root. 
	Cubing both sides we get 
	$$\begin{align} x + (2x-3) + 3x^\frac{1}{3}(2x-3)^\frac{1}{3}(x^\frac{1}{3}+(2x-3)^\frac{1}{3}) &= 12(x-1) \\
	            3x^\frac{1}{3}(2x-3)^\frac{1}{3}(12(x-1))^\frac{1}{3} = 9(x-1) \end{align}$$
	Cubing both sides again 
	$$ \begin{align} 27x(2x-3)12(x-1) &= 9^3(x-1)^3 \\
	                 4x(2x-3) &= 9(x-1)^2 \\
		  			 8x^2-12x  & = 9x^2-18x+9 \\
					 0 &= x^2 - 6x + 9 \\
	\end{align} $$
	The above equation has dual roots of $3,3$. Therefore $x=1,3,3$ are the roots of the equation