---
layout: post
tags: binomial
---

## Problem

Find the coefficient of $x^6$ in the expansion of $(1-3x)^\frac{10}{3}$, and the term independent of $x$ in $(\frac{4}{3}x^2-\frac{3}{2x})^9$.

## Solution

Coefficient of $x^6$ will be 

$$\begin{align} &= \frac{\frac{10}{3}(\frac{10}{3}-1)(\frac{10}{3}-2)(\frac{10}{3}-3)(\frac{10}{3}-4)(\frac{10}{3}-5)}{1.2.3.4.5.6} \\
             &= \frac{\frac{10}{3}\frac{7}{3}\frac{4}{3}\frac{1}{3}(-\frac{2}{3})(-\frac{5}{3})}{1.2.3.4.5.6} \\
			 &= \frac{10.7.4.1.(-2).(-5)}{3^6.1.2.3.4.5.6} \\
			 &= \frac{35}{3^8} \end{align} $$

The $(k+1)^{th}$ term of the expansion would be $\binom{9}{k}(\frac{4}{3}x^2)^{9-k}(-\frac{3}{2x})^k$. For this to be independent of $x$, the powers of $x$ in the 
numerator and denominator should cancel out which implies that $2(9-k)=k$ or $k=6$. and the coeffcient would be 

$$\begin{align} &= \binom{9}{6}(\frac{4}{3})^{9-6}(-\frac{3}{2})^6 \\
                &= \frac{9!}{6!3!} \frac{4^3}{3^3}\frac{3^6}{2^6} \\ 
				&= \frac{9.8.7}{3!}.3^3 \\
				&= 2268 \\
				\end{align} $$
