---
layout: post
tags: equations
---

## Problem

Eliminate $x,y,z$ between the equations:

$ x^2-yz=a^2, y^2-zx= b^2, z^2-xy = c^2, x+y+z=0 $ [R.M.A. WOOLWICH]

## Solution

Add the first two equations and subtract from twice the 3rd
  
$$ \begin{align}
     x^2-yz+y^2-zx-2(z^2-xy) &= a^2+b^2-2c^2 \\
	 x^2+y^2+2xy-2z^2-yz-zx &= a^2+b^2-2c^2 \\
	 (x+y)^2-2z^2-z(x+y) &= a^2+b^2-2c^2 \\
	 z^2-2z^2+z^2 &= a^2 + b^2-2c^2 \\
	 a^2+b^2-2c^2 &= 0 \end{align} $$
Similarly
  $b^2+c^2=2a^2$ and $a^2+c^2=2b^2$